#+OPTIONS: toc:nil
* Chapter Exercises:
** Combinators:
1. \( {\lambda}x.xxx \) -> Combinator
2. \( {\lambda}xy.zx\) -> Not Combinator
3. \( {\lambda}xyz.xy(zx) \) -> Combinator
4. \({\lambda}xyz.xy(zxy) \) -> Combinator
5. \( {\lambda}xy.xy(zxy)\) -> Not Combinator

** Normal form or diverge
1. \( {\lambda}x.xxx \) -> No further reductions possible so this is already in normal form
2. \( ({\lambda}z.zz) ({\lambda}y.yy)\)
   \([z := ({\lambda}y.yy)] \)
   \( ({\lambda}y.yy)({\lambda}y.yy)\)
   \([ y := ({\lambda}y.yy)] \)
   \(({\lambda}y.yy)({\lambda}y.yy)\)
   This will no longer reduce and will continue infinitely. So the expression is divergent
3. \(({\lambda}x.xxx)z\)
   \([x := z]\)
   \(zzz\)
   This has been reduced to normal form

** Beta reduction
1. \( ({\lambda}abc.cba) zz ({\lambda}wv.w) \)
   \( ({\lambda}a.{\lambda}b.{\lambda}c.cba) zz ({\lambda}wv.w) \)
   \( [a := z] \)
   \( ({\lambda}b.{\lambda}c.cbz) z ({\lambda}wv.w)\)
   \( [b := z] \)
   \( ({\lambda}c.czz) ({\lambda}wv.w) \)
   \( [c := ({\lambda}wv.w)] \)
   \( ({\lambda}wv.w) z z \)
   \( [ w := z] \)
   \( ({\lambda}v.z) \)
   \( [ v := z ] \)
   \( z \)
2. \( ({\lambda}x.{\lambda}y.xyy)({\lambda}a.a)b \)
   \( [x := ({\lambda}a.a)] \)
   \( ({\lambda}y({\lambda}a.a)yy)b \)
   \( [ y := ({\lambda}b.b)] \)
   \( ({\lambda}a.a)bb \)
   \( [ a := b ] \)
   \( bb \)
3. \( ({\lambda}y.y)({\lambda}x.xx)({\lambda}z.zq) \)
   \( [y := ({\lambda}x.xx)] \)
   \( ({\lambda}x.xx)({\lambda}z.zq) \)
   \( [x := ({\lambda}z.zq)] \)
   \( ({\lambda}z.zq)({\lambda}z.zq) \)
   \( [z := ({\lambda}z.zq)] \)
   \( ({\lambda}z.zq)q \)
   \([ z := q ]\)
   \( qq \)
4. \( ({\lambda}z.z)({\lambda}z.zz)({\lambda}z.zy) \)
   \( ({\lambda}z_1.z_1)({\lambda}z_2.z_2z_2)({\lambda}z_3.z_3y) \)
   \( [z_1 := ({\lambda}z_2.z_2z_2)] \)
   \(({\lambda}z_2.z_2z_2)({\lambda}z_3.z_3y)\)
   \( [z_2 := ({\lambda}z_3.z_3y)] \)
   \( ({\lambda}z_3.z_3y)({\lambda}z_3.z_3y) \)
   \( [z_3 := ({\lambda}z_3.z_3y)] \)
   \( ({\lambda}z_3.z_3y)y \)
   \( [ z_3 := y ] \)
   \( yy \)
5. \( ({\lambda}x.{\lambda}y.xyy)({\lambda}y.y)y \)
   \( ({\lambda}x.{\lambda}y_1.xy_1y_1)({\lambda}y_2.y_2)y_3 \)
   \([x := ({\lambda}y_2.y_2)] \)
   \( ({\lambda}y_1.({\lambda}y_2.y_2)y_1y_1)y_3 \)
   \( [ y_1 := y_3 ] \)
   \( ({\lambda}y_2y_2)y_3y_3 \)
   \( [y_2 := y_3] \)
   \(y_3y_3\)
